just trying to add some functions to set and map turns into a big refactoring (wip/does not compile)

bedrock2/src/FlatImp.v
@@ -1,6 +1,6 @@
 Require Import lib.LibTacticsMin.
 Require Import riscv.util.BitWidths.
-Require Import compiler.Common.
+Require Import compiler.util.Common.
 Require Import compiler.util.Tactics.
 Require Import compiler.Op.
 Require Import compiler.StateCalculus.
@@ -17,10 +17,10 @@ Section FlatImp1.
   Notation func := (@name FName).
   Existing Instance eq_name_dec.
 
-  Context {state: Type}.
-  Context {stateMap: Map state var (word wXLEN)}.
-  Context {vars: Type}.
-  Context {varset: set vars var}.
+  Context {stateMap: MapFunctions var (word wXLEN)}.
+  Notation state := (map var (word wXLEN)).
+  Context {varset: SetFunctions var}.
+  Notation vars := (set var).
 
   Ltac state_calc := state_calc_generic (@name Name) (word wXLEN).
 
@@ -37,7 +37,9 @@ Section FlatImp1.
     | SCall(binds: list var)(f: func)(args: list var).
 
   Section WithEnv.
-    Context {env} {funcMap: Map env func (list var * list var * stmt)} (e:env).
+    Context {funcMap: MapFunctions func (list var * list var * stmt)}.
+    Notation env := (map func (list var * list var * stmt)).
+    Context (e: env).
 
     (* If we want a bigstep evaluation relation, we either need to put
        fuel into the SLoop constructor, or give it as argument to eval *)
@@ -82,11 +84,11 @@ Section FlatImp1.
         | SCall binds fname args =>
           fimpl <- get e fname;
           let '(params, rets, fbody) := fimpl in
-          argvs <- option_all (map (get st) args);
-          st0 <- putmany params argvs empty;
+          argvs <- option_all (List.map (get st) args);
+          st0 <- putmany params argvs empty_map;
           st1m' <- eval_stmt f st0 m fbody;
           let '(st1, m') := st1m' in
-          retvs <- option_all (map (get st1) rets);
+          retvs <- option_all (List.map (get st1) rets);
           st' <- putmany binds retvs st;
           Return (st', m')
         end
@@ -165,10 +167,10 @@ Section FlatImp1.
       eval_stmt (S f) st m1 (SCall binds fname args) = Some p2 ->
       exists params rets fbody argvs st0 st1 m' retvs st',
         get e fname = Some (params, rets, fbody) /\
-        option_all (map (get st) args) = Some argvs /\
-        putmany params argvs empty = Some st0 /\
+        option_all (List.map (get st) args) = Some argvs /\
+        putmany params argvs empty_map = Some st0 /\
         eval_stmt f st0 m1 fbody = Some (st1, m') /\
-        option_all (map (get st1) rets) = Some retvs /\
+        option_all (List.map (get st1) rets) = Some retvs /\
         putmany binds retvs st = Some st' /\
         p2 = (st', m').
     Proof. inversion_lemma. Qed.
@@ -271,16 +273,17 @@ Section FlatImp2.
   Context {FName : NameWithEq}.
   Notation func := (@name FName).
 
-  Context {state: Type}.
-  Context {stateMap: Map state var (word wXLEN)}.
-  Context {vars: Type}.
-  Context {varset: set vars var}.
+  Context {stateMap: MapFunctions var (word wXLEN)}.
+  Notation state := (map var (word wXLEN)).
+  Context {varset: SetFunctions var}.
+  Notation vars := (set var).
 
-  Context {env} {funcMap: Map env func (list var * list var * stmt)}.
+  Context {funcMap: MapFunctions func (list var * list var * @stmt Bw Name FName)}.
+  Notation env := (map func (list var * list var * stmt)).
 
   Ltac state_calc := state_calc_generic (@name Name) (word wXLEN).
 
-  Lemma increase_fuel_still_Success: forall fuel1 fuel2 e initialSt initialM s final,
+  Lemma increase_fuel_still_Success: forall fuel1 fuel2 (e: env) initialSt initialM s final,
     fuel1 <= fuel2 ->
     eval_stmt e fuel1 initialSt initialM s = Some final ->
     eval_stmt e fuel2 initialSt initialM s = Some final.
@@ -365,10 +368,15 @@ Example fib(n: word 32) :=
          SSeq (SSet _b _s) (
               (SOp _n OMinus _n _one)))))
   )))).
+Set Printing Implicit.
 
-Definition eval_stmt_test fuel initialSt := @eval_stmt _ ZName ZName _ _ _ _ empty fuel initialSt no_mem.
+Definition annoying_eq: DecidableEq
+  (list (@name ZName) * list (@name ZName) * @stmt BitWidth32 ZName ZName). Admitted.
+Existing Instance annoying_eq.
 
-Example finalFibState(n: nat) := (eval_stmt_test 100 empty (fib $n)).
+Definition eval_stmt_test fuel initialSt := @eval_stmt BitWidth32 ZName ZName _ (List_Map _ _ (List_Set _)_) empty_map fuel initialSt no_mem.
+
+Example finalFibState(n: nat) := (eval_stmt_test 100 empty_map (fib $n)).
 Example finalFibVal(n: nat): option (word 32) := match finalFibState n with
 | Some (s, _) => get s _b
 | _ => None
