bedrock2/src/ExprImp.v
@@ -2,7 +2,7 @@ Require Import Coq.Lists.List.
 Import ListNotations.
 Require Import lib.LibTacticsMin.
 Require Import riscv.util.BitWidths.
-Require Import compiler.Common.
+Require Import compiler.util.Common.
 Require Import compiler.util.Tactics.
 Require Import compiler.Op.
 Require Import compiler.StateCalculus.
