bedrock2/src/util/Map.v
@@ -1,0 +1,52 @@
+Require Import compiler.util.Set.
+Require Import compiler.Decidable.
+Require Import Coq.Lists.List.
+
+Class MapFunctions(K V: Type) := mkMap {
+  map: Type;
+
+  map_domain_set: SetFunctions K;
+  map_range_set: SetFunctions V;
+
+  empty_map: map;
+  get: map -> K -> option V;
+  put: map -> K -> V -> map;
+  restrict: map -> set K -> map;
+  domain: map -> set K;
+  range: map -> set V;
+  
+  get_put_same: forall (m: map) (k: K) (v: V), get (put m k v) k = Some v;
+  get_put_diff: forall (m: map) (k1 k2: K) (v: V), k1 <> k2 -> get (put m k1 v) k2 = get m k2;
+  empty_is_empty: forall (k: K), get empty_map k = None
+
+  (* TODO probably needs some more properties *)
+}.
+
+Arguments map _ _ {_}.
+
+Definition TODO{T: Type}: T. Admitted.
+
+Instance List_Map(K V: Type)(domain_set: SetFunctions K)(range_set: SetFunctions V):
+  MapFunctions K V :=
+{|
+  map := list (K * V);
+  
+  map_domain_set := domain_set;
+  map_range_set := range_set;
+
+  empty_map := nil;
+  get A k := match find (fun a => if set_elem_eq_dec (fst a) k then true else false) A with
+             | Some (_, v) => Some v
+             | None => None
+             end;
+  put A k v := (fix rec A := match A with
+                            | (k1, v1) :: rest => if set_elem_eq_dec k1 k then (k, v) :: rest
+                                                 else (k1, v1) :: rec rest
+                            | nil => (k, v) :: nil
+                            end) A;
+  restrict M A := filter (fun p => containsb A (fst p)) M;
+  domain M := of_list (List.map fst M);
+  range M := of_list (List.map snd M);
+|}.
+all: apply TODO.
+Defined.
