bedrock2/src/util/Set.v
@@ -1,0 +1,87 @@
+Require Import compiler.util.Tactics.
+Require Import compiler.Decidable.
+Require Import compiler.util.ListLib.
+Require Import Coq.Program.Tactics.
+Require Import Coq.Lists.List.
+Import ListNotations.
+
+Class SetFunctions(E: Type) := mkSet {
+  set: Type;
+
+  contains: set -> E -> Prop;
+  containsb: set -> E -> bool;
+
+  empty_set: set;
+  singleton_set: E -> set;
+
+  union: set -> set -> set;
+  intersect: set -> set -> set;
+  diff: set -> set -> set;
+  pick_or_else: set -> E -> (E * set);
+
+  set_elem_eq_dec: DecidableEq E;
+  empty_set_spec: forall (x: E), contains empty_set x <-> False;
+  containsb_spec: forall (x: E) (A: set), containsb A x = true <-> contains A x;
+  singleton_set_spec: forall (x y: E), contains (singleton_set y) x <-> x = y;
+  union_spec: forall (x: E) (A B: set), contains (union A B) x <-> contains A x \/ contains B x;
+  intersect_spec: forall (x: E) (A B: set), contains (intersect A B) x <-> contains A x /\ contains B x;
+  diff_spec: forall (x: E) (A B: set), contains (diff A B) x <-> contains A x /\ ~ contains B x;
+  pick_or_else_spec: forall (A: set) (default: E),
+      A = empty_set /\ pick_or_else A default = (default, empty_set) \/
+      exists (a: E), contains A a /\ pick_or_else A default = (a, diff A (singleton_set a))
+}.
+
+Arguments set E {_}.
+
+Hint Rewrite
+  @empty_set_spec
+  @singleton_set_spec
+  @union_spec
+  @intersect_spec
+  @diff_spec
+: rew_set_op_specs.
+
+Notation "x '\in' s" := (contains s x) (at level 39, no associativity).
+
+Section SetDefinitions.
+  Context {E: Type}.
+  Context {setInst: SetFunctions E}.
+
+  Definition add(s: set E)(e: E) := union (singleton_set e) s.
+  Definition remove(s: set E)(e: E) := diff s (singleton_set e).
+  Definition subset(s1 s2: set E) := forall x, x \in s1 -> x \in s2.
+  Definition disjoint(s1 s2: set E) := forall x, (~ x \in s1) \/ (~ x \in s2).
+  Definition of_list l := List.fold_right union empty_set (List.map singleton_set l).
+End SetDefinitions.
+
+Hint Unfold add subset disjoint : unf_set_defs.
+
+Definition TODO{T: Type}: T. Admitted.
+
+Instance List_Set(E: Type){eeq: DecidableEq E}: SetFunctions E := {|
+  set := list E;
+
+  contains A e := List.In e A;
+  containsb A e := if List.in_dec eeq e A then true else false;
+
+  empty_set := nil;
+  singleton_set e := (cons e nil);
+
+  union := list_union;
+  intersect := list_intersect;
+  diff := list_diff;
+  pick_or_else A default := match A with
+                             | a :: rest => (a, rest)
+                             | nil => (default, nil)
+                            end;
+|}.
+all: apply TODO.
+Defined.
+
+Ltac set_solver_generic E :=
+  repeat autounfold with unf_set_defs in *;
+  destruct_products;
+  intros;
+  specialize_with E;
+  autorewrite with rew_set_op_specs in *;
+  intuition (subst *; auto).
